common/auxiliary.lean
@@ -1,5 +1,11 @@
 variables {α β γ : Type}
 
+lemma add_le_iff_le_sub (a b c : int) : a + b ≤ c ↔ a ≤ c - b := 
+iff.intro (le_sub_right_of_add_le) (add_le_of_le_sub_right)
+
+lemma add_left [has_add α] {a b c : α} (h : b = c) : a + b = a + c := 
+h ▸ eq.refl _
+
 lemma le_iff_add_le_add_right [ordered_cancel_comm_monoid α] (a b c : α) : 
 (a ≤ b) ↔ (a + c ≤ b + c) := 
 begin 
@@ -7,63 +13,6 @@ begin
   intros h, apply add_le_add_right h,
   apply le_of_add_le_add_right h
 end
-
-
-def list.sum [has_zero α] [has_add α] : list α → α 
-| [] := @has_zero.zero α _
-| (a::as) := a + list.sum as
-
-lemma zip_nil (as : list α) : list.zip as ([] : list β) = [] :=
-begin
-  cases as with a as, 
-  unfold list.zip, unfold list.zip_with, 
-  unfold list.zip, unfold list.zip_with 
-end
-
-lemma exp_zip (a) (as : list α) (b) (bs : list β) : 
-  list.zip (a::as) (b::bs) = (a,b)::(list.zip as bs) :=
-begin unfold list.zip, unfold list.zip_with end
-
-def dot_prod [has_zero α] [has_add α] [has_mul α] (as1 as2 : list α) : α := 
-list.sum (list.map (λ xy, prod.fst xy * prod.snd xy) (list.zip as1 as2))
-
-lemma nil_dot_prod [has_zero α] [has_add α] [has_mul α] (as : list α) : 
-dot_prod [] as = 0 := 
-begin
-  unfold dot_prod, unfold list.zip, 
-  unfold list.zip_with, simp, unfold list.sum
-end
-
-lemma dot_prod_nil [has_zero α] [has_add α] [has_mul α] (as : list α) : 
-dot_prod as [] = 0 := 
-begin
-  unfold dot_prod, rewrite zip_nil, 
-  simp, unfold list.sum
-end
-
-lemma exp_dot_prod [has_zero α] [has_add α] [has_mul α] (a1 a2 : α) (as1 as2 : list α) : 
-dot_prod (a1::as1) (a2::as2) = (a1 * a2) + dot_prod as1 as2 := 
-begin
-  unfold dot_prod, rewrite exp_zip,
-  simp, unfold list.sum
-end
-
-meta def exp_neg_dot_prod_aux : tactic unit := 
-`[unfold dot_prod, simp, unfold list.zip, unfold list.zip_with, 
-  simp, unfold list.sum] 
-
-def exp_neg_dot_prod [ring α] : ∀ (as1 as2 : list α),  
-  dot_prod (list.map has_neg.neg as1) as2 = has_neg.neg (dot_prod as1 as2) 
-| [] []      := begin exp_neg_dot_prod_aux, rewrite neg_zero end 
-| (a::as) [] := begin exp_neg_dot_prod_aux, rewrite neg_zero end 
-| [] (a::as) := begin exp_neg_dot_prod_aux, rewrite neg_zero end 
-| (a1::as1) (a2::as2) := 
-  begin 
-    exp_neg_dot_prod_aux, 
-    have hrw := (exp_neg_dot_prod as1 as2),
-    unfold dot_prod at hrw, unfold list.zip at hrw, 
-    simp, rewrite hrw, 
-  end
 
 lemma iff_of_eq {p q} : p = q → (p ↔ q) :=
 begin intro h, rewrite h end
@@ -80,29 +29,6 @@ begin
   exfalso, apply h hd
 end
 
-def list.omap (f : α → option β) : list α → list β  
-| [] := []
-| (a::as) := 
-  match f a with 
-  | none := list.omap as 
-  | (some b) := b::(list.omap as) 
-  end
-
-lemma exp_mem_cons {a' a : α} {as} : a' ∈ a::as ↔ (a' = a ∨ a' ∈ as) := 
-by {unfold has_mem.mem, unfold list.mem}
-
-lemma exp_mem_nil {a : α} : (a ∈ ([] : list α)) ↔ false := 
-begin
-  apply iff.intro; intro h, cases h, 
-  exfalso, apply h
-end
-
-lemma exp_mem_singleton {a' a : α} : a' ∈ [a] ↔ (a' = a) := 
-begin
-  rewrite exp_mem_cons, rewrite exp_mem_nil,  
-  rewrite or_false
-end
-
 lemma exp_forall_eq {P : α → Prop} {a' : α} : 
   (∀ a, a = a' → P a) ↔ P a' := 
 begin
@@ -111,10 +37,6 @@ begin
   subst ha', apply h 
 end
 
-lemma eq_nil_of_map_eq_nil {f : α → β} {as}  
-  (h : list.map f as = []) : as = [] :=
-begin cases as, refl, cases h end
-
 def converse_linear_order (hlo : linear_order β) : linear_order β := 
 { le := λ x y, x ≥ y,
   le_refl := preorder.le_refl, 
@@ -122,237 +44,16 @@ def converse_linear_order (hlo : linear_order β) : linear_order β :=
   le_antisymm := λ x y hxy hyx, partial_order.le_antisymm _ _ hyx hxy,
   le_total := λ x y, linear_order.le_total _ _ }
 
-lemma exists_maximum [linear_order β] : 
-∀ (bs : list β) (hi : bs ≠ []), ∃ b, b ∈ bs ∧ ∀ b' ∈ bs, b' ≤ b 
-| [] hi := begin exfalso, apply hi rfl end
-| [b] hi := 
-  begin
-    existsi b, apply and.intro (or.inl rfl), 
-    intros b' hb', cases hb' with hb' hb', 
-    subst hb', cases hb',
-  end
-| (b::b'::bs') hi := 
-  begin
-    cases (exists_maximum (b'::bs') _) with bm hbm, 
-    cases hbm with hbm1 hbm2,
-    apply @classical.by_cases (b ≤ bm); intro hle,
-
-    existsi bm, apply and.intro (or.inr hbm1), 
-    intros bl hbl, rewrite exp_mem_cons at hbl, 
-    cases hbl with hbl hbl, subst hbl, apply hle, 
-    apply hbm2 _ hbl,
-
-    existsi b, apply and.intro (or.inl rfl),
-    intros bl hbl, rewrite exp_mem_cons at hbl, 
-    cases hbl with hbl hbl, subst hbl, 
-    apply le_trans, apply hbm2 _ hbl, 
-    apply le_of_not_le hle, 
-    intro hc, cases hc 
-  end
-
-lemma exists_minimum [hlo : linear_order β] : 
-∀ (bs : list β) (hi : bs ≠ []), ∃ b, b ∈ bs ∧ ∀ b' ∈ bs, b' ≥ b :=  
-@exists_maximum _ (converse_linear_order hlo)
-
-lemma mem_omap {f : α → option β} {a} {b} (he : f a = some b) : 
-  ∀ {as : list α} (HM : a ∈ as), b ∈ list.omap f as  
-| [] hm := by cases hm
-| (a'::as) hm :=
-  begin 
-    unfold has_mem.mem at hm, unfold list.mem at hm,
-    cases hm with hm hm, subst hm,
-    unfold list.omap, rewrite he, apply or.inl rfl,
-    unfold list.omap, cases (f a'), 
-    apply mem_omap, apply hm, 
-    apply or.inr, apply mem_omap, apply hm 
-  end 
-
-lemma mem_omap_of_mem_omap_tail {f : α → option β} {a} {b} :
-  ∀ {as : list α}, b ∈ list.omap f as → b ∈ list.omap f (a::as) := 
-begin
-  intros as h, unfold list.omap, cases (f a),
-  apply h, apply or.inr h
-end
 
 lemma dest_option : ∀ (o : option α), o = none ∨ ∃ a, o = some a  
 | none := or.inl rfl 
 | (some a) := begin apply or.inr, existsi a, refl end
-
-lemma dest_list : ∀ (as : list α), as = [] ∨ ∃ a' as', as = (a'::as')
-| [] := or.inl rfl 
-| (a::as) := begin apply or.inr, existsi a, existsi as, refl end
-
-lemma exp_mem_omap {f : α → option β} {b : β} : ∀ {as : list α}, (b ∈ list.omap f as) ↔ ∃ a, a ∈ as ∧ some b = f a 
-| [] := 
-  iff.intro 
-    (by {intro h, cases h}) 
-    (begin intro h, cases h with a ha, cases ha^.elim_left end)
-| (a::as) := 
- iff.intro 
- (begin
-    intro h, unfold list.omap at h, 
-    cases (dest_option (f a)) with ho ho, 
-    rewrite ho at h, 
-    cases (exp_mem_omap^.elim_left h) with a' ha', 
-    cases ha' with ha1' ha2',
-    existsi a', apply and.intro (or.inr ha1') ha2',
-    cases ho with b' hb', rewrite hb' at h,
-    unfold list.omap at h, rewrite exp_mem_cons at h,
-    cases h with h h, existsi a,
-    apply and.intro (or.inl rfl), rewrite h,
-    apply eq.symm hb',
-    cases (exp_mem_omap^.elim_left h) with a' ha', 
-    cases ha' with ha1' ha2',
-    existsi a', apply and.intro (or.inr ha1') ha2'
-  end)
- (begin 
-   intro h, cases h with a' ha', 
-   cases ha' with h1 h2, rewrite exp_mem_cons at h1, 
-   cases h1 with h1 h1, 
-   unfold list.omap, subst h1, rewrite eq.symm h2, 
-   apply or.inl rfl, apply mem_omap_of_mem_omap_tail,
-   apply exp_mem_omap^.elim_right, existsi a',
-   apply and.intro h1 h2
-  end)
-
-def list.product : list α → list β → list (α × β) 
-| [] _ := []
-| (a1::l1) l2 := (list.map (λ a2, ⟨a1,a2⟩) l2) ++ list.product l1 l2 
-
-lemma product_nil : ∀ {l : list α}, list.product l (@list.nil β) = [] 
-| [] := by unfold list.product   
-| (a::as) := 
-  begin unfold list.product, rewrite product_nil, simp, end
-
-def list.first (p : α → Prop) [decidable_pred p] : list α → option (α × list α)
-| []      := none 
-| (a::as) := 
-  if p a 
-  then some (a, as) 
-  else do (a',as') ← list.first as, 
-          some (a',a::as')
 
 lemma cases_ite {P} {Q : α → Prop} {HD : decidable P} {f g : α} 
   (Hf : P → Q f) (Hg : ¬ P → Q g) : Q (@ite P HD α f g) := 
 begin
   unfold ite, cases HD with h h, simp, apply Hg h,
   simp, apply Hf h
-end
-
-def exp_mem_insert [hd : decidable_eq α] {a1 a2 : α} {as : list α} :
-  a1 ∈ (list.insert a2 as) ↔ (a1 = a2 ∨ a1 ∈ as) := 
-begin
-  unfold list.insert,  
-  apply @cases_ite _ (a2 ∈ as) 
-    (λ as', a1 ∈ as' ↔ a1 = a2 ∨ a1 ∈ as)
-    _ as _; intro h1; apply iff.intro; intro h2,
-  apply or.inr h2,
-  cases h2 with h2 h2, subst h2, apply h1, apply h2,
-  rewrite exp_mem_cons at h2, apply h2,    
-  rewrite exp_mem_cons, apply h2 
-end
-
-meta def unfold_list_union := 
-`[unfold has_union.union, unfold list.union, unfold list.foldr] 
-
-/-
-def mem_or_mem_of_mem_union [decidable_eq α] (a : α) : 
-  ∀ (as1 as2 : list α), a ∈ (as1 ∪ as2) → (a ∈ as1 ∨ a ∈ as2)  
-| [] as2 := 
-  begin
-    unfold_list_union, 
-    intro h, apply or.inr h
-  end
-| (a1::as1) as2 :=
-  begin
-    unfold_list_union, intro h,
-  end -/
-
-lemma exp_cons_union [decidable_eq α] (a : α) (as1 as2) : 
-  (a::as1) ∪ as2 = list.insert a (as1 ∪ as2) := rfl
-
-lemma mem_union_of_mem_left [decidable_eq α] {a : α} : 
-  ∀ {as1 as2 : list α}, (a ∈ as1) → a ∈ (as1 ∪ as2)  
-| [] as2 hm := by cases hm
-| (a1::as1) as2 hm := 
-  begin
-    rewrite exp_mem_cons at hm,
-    rewrite exp_cons_union, 
-    rewrite exp_mem_insert, 
-    cases hm with hm hm,
-    apply or.inl hm, 
-    apply or.inr (mem_union_of_mem_left hm) 
-  end
-
-lemma mem_union_of_mem_right [decidable_eq α] {a : α} : 
-  ∀ {as1 as2 : list α}, (a ∈ as2) → a ∈ (as1 ∪ as2)  
-| [] as2 hm := hm
-| (a1::as1) as2 hm := 
-  begin
-    rewrite exp_cons_union, rewrite exp_mem_insert, 
-    apply or.inr, apply mem_union_of_mem_right hm
-  end
-
-lemma mem_union_of_mem_either [decidable_eq α] {a : α}  
-  {as1 as2 : list α} (h : a ∈ as1 ∨ a ∈ as2) : a ∈ (as1 ∪ as2) := 
-begin
-  cases h with h h, 
-  apply mem_union_of_mem_left h, 
-  apply mem_union_of_mem_right h 
-end
-
-lemma mem_either_of_mem_union [decidable_eq α] {a : α} : 
-  ∀ {as1 as2 : list α} (hm : a ∈ (as1 ∪ as2)), a ∈ as1 ∨ a ∈ as2 
-| [] as2 hm := or.inr hm  
-| (a1::as1) as2 hm := 
-  begin
-    rewrite exp_cons_union at hm,
-    rewrite exp_mem_insert at hm, 
-    cases hm with hm hm, 
-    apply or.inl (or.inl hm),
-    cases (mem_either_of_mem_union hm) with hm' hm',
-    apply or.inl (or.inr hm'),
-    apply or.inr hm'
-  end
-
-lemma exp_mem_union[decidable_eq α] {a : α}  {as1 as2 : list α} :
-  (a ∈ as1 ∪ as2) ↔ (a ∈ as1 ∨ a ∈ as2) := 
-  iff.intro mem_either_of_mem_union mem_union_of_mem_either
-
-def list.eqmem (l1 l2 : list α) := ∀ (a : α), (a ∈ l1 ↔ a ∈ l2)
-
-def eqmem_refl {l : list α} : list.eqmem l l := λ a, iff.refl _
-
-lemma eqmem_trans {l1 l2 l3 : list α} : list.eqmem l1 l2 → list.eqmem l2 l3 → list.eqmem l1 l3 :=  
-begin
-  intros H1 H2, intro x, apply iff.trans,
-  apply H1, apply H2
-end 
-
-lemma eqmem_swap {a1 a2 : α} {l} : list.eqmem (a1::a2::l) (a2::a1::l) :=  
-begin
-  intro a, apply iff.intro, 
-  intro H, cases H with H H, subst H, 
-  apply or.inr, apply or.inl, refl,
-  cases H with H H, subst H, 
-  apply or.inl, refl,
-  apply or.inr, apply or.inr, apply H,
-  intro H, cases H with H H, subst H, 
-  apply or.inr, apply or.inl, refl,
-  cases H with H H, subst H, 
-  apply or.inl, refl,
-  apply or.inr, apply or.inr, apply H,
-end
-
-lemma eqmem_cons {a : α} {l1 l2} : list.eqmem l1 l2 → list.eqmem (a::l1) (a::l2) := 
-begin
-  intros H a', apply iff.intro, 
-  intro HM, cases HM with HM HM, 
-  apply or.inl HM, apply or.inr, 
-  apply (H a')^.elim_left, apply HM,
-  intro HM, cases HM with HM HM, 
-  apply or.inl HM, apply or.inr, 
-  apply (H a')^.elim_right, apply HM,
 end
 
 lemma true_iff_true {p q} : p → q → (p ↔ q) := 
@@ -365,45 +66,6 @@ begin
   intro hq, apply absurd hq hnq
 end
 
-def allp (P : α → Prop) (l : list α) := ∀ a, a ∈ l → P a
-
-def anyp (P : α → Prop) (l : list α) := ∃ a, a ∈ l ∧ P a
-
-lemma allp_nil {P : α → Prop} : allp P [] :=
-begin intros _ H, cases H end
-
-lemma allp_of_allp_cons {P : α → Prop} {a} {as} (h : allp P (a::as)) : 
-  allp P as :=
-begin intros a' ha', apply h, apply or.inr ha' end
-
-lemma exp_allp_nil {P : α → Prop} : allp P [] ↔ true :=
-true_iff_true allp_nil trivial
-
-lemma allp_of_allp {P Q : α → Prop} (H : ∀ a, P a → Q a) 
-  (as) (HP : allp P as) : allp Q as :=
-begin intros a Ha, apply H, apply HP, apply Ha end
-
-lemma allp_union_of_allp_both [decidable_eq α] {P : α → Prop} {as1 as2}  
-  (h : allp P as1 ∧ allp P as2) : allp P (as1 ∪ as2) :=
-begin
-  cases h with h1 h2, intros a ha, 
-  rewrite exp_mem_union at ha, 
-  cases ha with ha ha, 
-  apply h1 _ ha, apply h2 _ ha,
-end
-
-lemma allp_both_of_allp_union [decidable_eq α] {P : α → Prop} {as1 as2}  
-  (h : allp P (as1 ∪ as2)) : allp P as1 ∧ allp P as2 :=
-begin
-  apply and.intro; intros a ha; apply h,
-  apply mem_union_of_mem_left ha,
-  apply mem_union_of_mem_right ha
-end
-
-lemma exp_allp_union [decidable_eq α] (P : α → Prop) (as1 as2) :
-  (allp P (as1 ∪ as2)) ↔ (allp P as1 ∧ allp P as2) :=
-iff.intro allp_both_of_allp_union allp_union_of_allp_both
-
 lemma eq_true_or_eq_false_of_dec (P) [HP : decidable P] : P = true ∨ P = false :=
 begin
   cases HP, 
@@ -411,302 +73,11 @@ begin
   apply or.inl, rewrite eq_true, simp *,
 end
 
-def dec_allp {P : α → Prop} [HP : decidable_pred P] : decidable_pred (allp P)  
-| [] := is_true (by apply allp_nil)
-| (a::as) := 
-  begin
-    cases (HP a) with HP HP, apply is_false, intro HC,  
-    apply absurd (HC a (or.inl (by refl))) HP,
-    cases (dec_allp as) with Has Has, 
-    apply is_false, intro HC, apply Has, 
-    intros x Hx, apply HC, apply or.inr Hx, 
-    apply is_true, intros x Hx, cases Hx with Hx Hx,
-    rewrite Hx, apply HP, apply Has x Hx 
-  end
-
-lemma cases_first (P : α → Prop) [HD : decidable_pred P] : ∀ (as : list α), 
-(list.first P as = none ∧ allp (λ x, ¬ P x) as) 
-∨ ∃ (a) (as'), (list.first P as = some (a,as') ∧ P a ∧ list.eqmem as (a::as'))
-| [] := 
-  begin 
-    apply or.inl, apply and.intro, 
-    unfold list.first, intros _ H, cases H
-  end
-| (a::as) :=
-  begin
-    repeat {unfold list.first, unfold ite}, simp,
-    cases (HD a) with Ha Ha, simp, 
-    cases (cases_first as) with Has Has,  
-    cases Has with Has1 Has2, 
-    apply or.inl, apply and.intro, 
-    intros x Hx, cases Hx with Hx Hx,
-    rewrite Hx, apply Ha, apply Has2, apply Hx,
-    rewrite Has1, refl, 
-    cases Has with x Has, cases Has with xs Hx,  
-    apply or.inr, existsi x, existsi (a::xs),
-    cases Hx with Hx1 Hx, cases Hx with Hx2 Hx3, 
-    apply and.intro, apply Hx2, 
-    apply and.intro, 
-    apply eqmem_trans _ eqmem_swap,
-    apply eqmem_cons Hx3, rewrite Hx1,
-    refl, apply or.inr, existsi a, existsi as,
-    apply and.intro Ha, apply and.intro, 
-    apply eqmem_refl, simp
-  end
-
-@[simp] def list.nth_dft (a : α) (l : list α) (n : nat) : α :=  
-match list.nth l n with 
-| none := a 
-| (some a') := a'
-end
-
-def list.head_dft (a' : α) : list α → α 
-| [] := a'
-| (a::as) := a 
-
-lemma nth_pred (a : α) (l : list α) (n : nat) (H : n > 0) : 
-list.nth (a::l) n = list.nth l (n - 1) := 
-begin cases n, cases H, simp end
-
-lemma nth_dft_pred {a a' : α} {l : list α} {n : nat} (H : n > 0) : 
-list.nth_dft a (a'::l) n = list.nth_dft a l (n - 1) :=
-begin unfold list.nth_dft, rewrite nth_pred, apply H  end
-
-lemma nth_dft_succ {a a' : α} {l : list α} {n : nat} : 
-list.nth_dft a (a'::l) (n+1) = list.nth_dft a l n :=
-begin unfold list.nth_dft, simp  end
-
-
-lemma nth_dft_head {a a' : α} {as : list α} : list.nth_dft a' (a::as) 0 = a := 
-begin unfold list.nth_dft, simp end
-
-def append_pair {α : Type} : (list α × list α) → list α  
-| (l1,l2) := l1 ++ l2 
-
-def all_true (ps : list Prop) : Prop := ∀ (p : Prop), p ∈ ps → p
-
-lemma all_true_nil : all_true [] := 
-by {intros _ H, cases H}
-
-def disj_list : list Prop → Prop 
-| [] := false
-| (p::ps) := p ∨ disj_list ps
-
-def some_true (ps : list Prop) : Prop := ∃ (p : Prop), p ∈ ps ∧ p
-
-lemma some_true_iff_disj_list : 
-  ∀ {ps : list Prop}, some_true ps ↔ disj_list ps 
-| [] :=
-  begin 
-    unfold some_true, unfold disj_list, 
-    apply iff.intro; intro h, cases h with x hx,
-    cases hx^.elim_left, exfalso, apply h
-  end
-| (p::ps) := 
-  begin
-    unfold some_true, unfold disj_list, 
-    apply iff.intro; intro h, cases h with x hx,
-    cases hx with hx1 hx2, rewrite exp_mem_cons at hx1,
-    cases hx1 with hx1 hx1, subst hx1, apply or.inl hx2, 
-    rewrite iff.symm some_true_iff_disj_list,
-    apply or.inr, existsi x, apply and.intro hx1 hx2,
-    cases h with h h, existsi p, 
-    apply and.intro (or.inl rfl) h, 
-    rewrite iff.symm some_true_iff_disj_list at h,
-    cases h with x hx, existsi x, cases hx with hx1 hx2,
-    apply and.intro (or.inr hx1) hx2 
-  end
-
-lemma disj_list_iff_some_true : ∀ (ps : list Prop), disj_list ps ↔ some_true ps 
-| [] := 
-  begin
-    apply iff.intro, intro H, cases H, 
-    intro H, cases H with H1 H2, cases (H2^.elim_left) 
-  end
-| (p::ps) :=
-  begin
-    apply iff.intro, intro H, cases H with H H, 
-    existsi p, apply and.intro, 
-    apply or.inl (eq.refl _), apply H, 
-    cases ((disj_list_iff_some_true ps)^.elim_left H) with p Hp,
-    existsi p, apply and.intro, 
-    apply or.inr (Hp^.elim_left),
-    apply Hp^.elim_right, 
-    unfold some_true, unfold disj_list,
-    unfold has_mem.mem, unfold list.mem,
-    intro H, cases H with p' Hp', 
-    cases (Hp'^.elim_left) with HM HM,
-    apply or.inl, rewrite (eq.symm HM), 
-    apply Hp'^.elim_right, 
-    apply or.inr, rewrite disj_list_iff_some_true,
-    existsi p', apply (and.intro HM Hp'^.elim_right)
-
-  end
-
-lemma mem_append_of_mem_or_mem : ∀ {l1 l2 : list α} {a : α}, a ∈ l1 ∨ a ∈ l2 → a ∈ (l1 ++ l2)  
-| [] l2 a := 
-  begin intro H, cases H with H H, cases H, simp, apply H end
-| (a'::l1) l2 a:= 
-  begin
-    unfold has_mem.mem, unfold list.mem, intro H, 
-    cases H with H H, cases H with H1 H2, 
-    apply or.inl, apply H1, 
-    apply or.inr, 
-    apply mem_append_of_mem_or_mem,
-    apply or.inl, apply H2, 
-    apply or.inr, 
-    apply mem_append_of_mem_or_mem,
-    apply or.inr, apply H 
-  end
-
-lemma mem_or_mem_of_mem_append : ∀ {l1 l2 : list α} {a : α}, a ∈ (l1 ++ l2) → a ∈ l1 ∨ a ∈ l2 
-| [] l2 a H := 
-  begin 
-    apply or.inr, apply H 
-  end
-| (a'::l1) l2 a H := 
-  begin 
-    cases H with H H, 
-    apply or.inl, apply or.inl, apply H, 
-    cases (mem_or_mem_of_mem_append H) with H1 H1 ; clear H,
-    apply or.inl, apply or.inr H1,
-    apply or.inr H1
-  end
-
-lemma disj_list_dist_append (l1 l2 : list Prop) : disj_list (l1 ++ l2) = (disj_list l1 ∨ disj_list l2) :=  
-begin
-  repeat {rewrite disj_list_iff_some_true}, 
-  apply propext, apply iff.intro,
-  intro H, cases H with x Hx, 
-  cases Hx with Hl Hr, cases (mem_or_mem_of_mem_append Hl) with HM HM, 
-  apply or.inl, existsi x, apply and.intro HM Hr,
-  apply or.inr, existsi x, apply and.intro HM Hr,
-  intro H, cases H with H H; cases H with x Hx ; cases Hx with Hl Hr ; existsi x ; apply and.intro, 
-  apply mem_append_of_mem_or_mem, 
-  apply or.inl, apply Hl, apply Hr, 
-  apply mem_append_of_mem_or_mem, 
-  apply or.inr, apply Hl, apply Hr 
-end
-
-def ex_arg_of_mem_map {f : α → β} {b : β} : 
-  ∀ {as : list α}, (b ∈ list.map f as) → ∃ a, a ∈ as ∧ b = f a 
-| [] H := by cases H 
-| (a::as) H := 
-  begin
-    simp at H, cases H with H H, existsi a, 
-    apply and.intro (or.inl (eq.refl _)) H,  
-    cases (ex_arg_of_mem_map H) with a' Ha',
-    existsi a', apply and.intro, 
-    apply or.inr (Ha'^.elim_left), 
-    apply Ha'^.elim_right
-  end
-
-lemma fst_mem_of_mem_product : 
-  ∀ {as : list α} {bs : list β} {p : α × β}, 
-    p ∈ (list.product as bs) → (prod.fst p) ∈ as  
-| [] bs b H := begin unfold list.product at H, cases H end
-| (a::as) bs b H := 
-  begin
-    unfold list.product at H, simp at H, cases H with H H,
-    apply or.inr, apply fst_mem_of_mem_product, apply H,
-    cases (ex_arg_of_mem_map H) with x Hx, 
-    rewrite Hx^.elim_right, apply or.inl, refl
-  end
-
-lemma snd_mem_of_mem_product : 
-  ∀ {as : list α} {bs : list β} {p : α × β}, 
-    p ∈ (list.product as bs) → (prod.snd p) ∈ bs 
-| [] bs b H := begin unfold list.product at H, cases H end
-| (a::as) bs b H := 
-  begin
-    unfold list.product at H, simp at H, cases H with H H,
-    apply snd_mem_of_mem_product, apply H,
-    cases (ex_arg_of_mem_map H) with x Hx, 
-    rewrite Hx^.elim_right, apply Hx^.elim_left
-  end
-
-def mem_map_of_mem {f : α → β} : ∀ {as : list α} {a : α}, a ∈ as → (f a) ∈ list.map f as 
-| [] a H := by cases H 
-| (a'::as) a H := 
-  begin
-    unfold list.map, cases H with H H,
-    rewrite H, apply or.inl (eq.refl _),
-    apply or.inr, apply @mem_map_of_mem as a H
-  end
-
-def mem_map_of_ex_arg {f : α → β} {b : β} : 
-  ∀ {as : list α}, (∃ a, a ∈ as ∧ b = f a) → b ∈ list.map f as := 
-begin
-  intros as hex, cases hex with a ha,
-  cases ha with ha1 ha2, subst ha2,
-  apply mem_map_of_mem ha1,
-end
-
-def exp_mem_map {f : α → β} {b : β} {as : list α} : 
- (b ∈ list.map f as) ↔ (∃ a, a ∈ as ∧ b = f a) :=
-iff.intro (ex_arg_of_mem_map) (mem_map_of_ex_arg)
-
-lemma mem_product_of_mem_of_mem :
-  ∀ {as : list α} {bs : list β} {a : α} {b : β}, 
-    a ∈ as → b ∈ bs → (a,b) ∈ list.product as bs 
-| [] _ _ _ H _ := by cases H
-| _ [] _ _ _ H := by cases H
-| (a::as) (b::bs) a' b' Ha Hb := 
-  begin
-    unfold has_mem.mem at Ha, unfold list.mem at Ha, 
-    unfold has_mem.mem at Hb, unfold list.mem at Hb, 
-    unfold has_mem.mem, unfold list.product, unfold list.map, 
-    unfold append, simp, unfold list.mem,
-    cases Ha with Ha Ha, cases Hb with Hb Hb, 
-    apply or.inl, simp *, 
-    apply or.inr, apply mem_append_of_mem_or_mem,
-    apply or.inl, simp *, apply mem_map_of_mem, 
-    apply Hb, apply or.inr, apply mem_append_of_mem_or_mem,
-    apply or.inr, apply mem_product_of_mem_of_mem,
-    apply Ha, apply Hb
-  end
-
-lemma map_dist_append {f : α → β} : 
-  ∀ (l1 l2 : list α), list.map f (l1 ++ l2) = (list.map f l1) ++ (list.map f l2) := 
-begin
-  intro l1, induction l1, intro l2, simp *,
-  intro l2, rename a_1 l1,
-  repeat {unfold append, unfold list.append}, 
-  repeat {unfold list.map}, unfold list.append,
-  apply congr_arg (list.cons (f a)), apply ih_1
-end
-
-def mem_filter_of_pred_and_mem {P : α → Prop} [HD : decidable_pred P] : ∀ (as : list α) (a : α), P a → a ∈ as → a ∈ list.filter P as 
-| [] a HP HM := by cases HM 
-| (a'::as) a HP HM := 
-  begin
-    unfold list.filter, unfold ite, 
-    unfold has_mem.mem at HM, unfold list.mem at HM,
-    cases HM with HM HM, 
-    cases (HD a') with HD HD, 
-    exfalso, apply HD, rewrite HM at HP, apply HP,
-    simp, apply or.inl HM,  
-    cases (HD a') with HD HD, simp, 
-    apply mem_filter_of_pred_and_mem, apply HP, 
-    apply HM, simp, 
-    apply or.inr, apply mem_filter_of_pred_and_mem,
-    apply HP, apply HM
-  end
-
 lemma map_compose (f : α → β) (g : β → γ) : ∀ (as : list α), list.map g (list.map f as) = list.map (λ x, g (f x)) as 
 | [] :=eq.refl _
 | (a::as) := by simp 
 
 lemma exp_compose (f : α → β) (g : β → γ) (a : α) : (λ x, g (f x)) a = g (f a) := eq.refl _ 
-
-lemma map_eq (f g : α → β)  : ∀ (as : list α) (H : ∀ a, a ∈ as → f a = g a), list.map f as = list.map g as 
-| [] _ := eq.refl _
-| (a::as) H := 
-  begin 
-    unfold list.map, rewrite H, rewrite map_eq,
-    intros a Ha, apply (H _ (or.inr Ha)),  
-    apply (or.inl (eq.refl _))
-  end
 
 def dec_not_pred_of_dec_pred (P : α → Prop) [H : decidable_pred P] : decidable_pred (λ x, ¬ P x) := 
 begin
@@ -714,21 +85,6 @@ begin
   apply decidable.is_true H, 
   apply decidable.is_false (not_not_intro H)
 end
-
-open tactic
-
-meta def papply pe := to_expr pe >>= apply  
-
-meta def intro_fresh : tactic expr :=
-get_unused_name `h none >>= tactic.intro 
-
-meta def intro_refl : tactic unit := 
-do t ← target, 
-   match t with 
-   | `(_ = _) := papply ``(eq.refl _)
-   | `(_ → _) := intro_fresh >> intro_refl
-   | _ := failed 
-   end
 
 lemma iff_not_not {p : Prop} : p ↔ ¬¬p := 
 iff.intro (not_not_intro) (classical.by_contradiction)
@@ -746,59 +102,6 @@ lemma iff_not_or {p q : Prop} : ¬ p ∧ ¬ q ↔ ¬(p ∨ q) :=
 iff.intro 
   (λ H, not_or H^.elim_left H^.elim_right)
   (λ H, and.intro (λ Hp, H $ or.inl Hp) (λ Hq, H $ or.inr Hq)) 
-
-meta def first_arg (f : α → tactic β) : list α → tactic β 
-| [] := failed 
-| (a::as) := f a <|> (first_arg as)
-
-meta def papply_trans (pe : pexpr) := 
-do papply ``(eq.trans), papply pe
-
-
-lemma eq_of_mem_singleton {a a' : α} : a ∈ [a'] → a = a' :=
-begin unfold has_mem.mem, unfold list.mem, rewrite or_false, apply id end
-
-lemma mem_of_mem_filter {P : α → Prop} {a : α} : 
-  ∀ {l : list α} {HD : decidable_pred P}, a ∈ (@list.filter _ P HD l) → a ∈ l  
-| [] _ := by {intro H, cases H} 
-| (a'::as) HD := 
-  begin
-    unfold list.filter, unfold ite, 
-    cases (HD a') with HD HD, simp, intro HM, 
-    apply or.inr, apply mem_of_mem_filter HM,
-    simp, intro HM, cases HM with H1 H2, 
-    apply or.inl H1, apply or.inr, 
-    apply mem_of_mem_filter H2,
-  end 
-
-lemma allp_filter_cond (P : α → Prop) [H : decidable_pred P] : ∀ (l : list α) , allp P (list.filter P l) 
-| [] := begin intros _ Ha, cases Ha end 
-| (x::xs) := 
-  begin 
-    unfold list.filter, unfold ite, 
-    cases (H x) with H1 H1, simp, apply allp_filter_cond, 
-    simp, intros a Ha, cases Ha with H2 H3, rewrite H2,
-    apply H1, apply allp_filter_cond, apply H3
-  end
-
-lemma allp_filter_of_allp {P Q : α → Prop} [H : decidable_pred Q] 
-  {as : list α} (h : allp P as) : allp P (list.filter Q as) := 
-begin
-  intros a ha, apply h, 
-  apply mem_of_mem_filter ha 
-end
-
-lemma pred_of_mem_filter_pred {P : α → Prop} {a : α} : 
-  ∀ {l : list α} {HD : decidable_pred P}, a ∈ (@list.filter _ P HD l) → P a 
-| [] HD := by {intro H, cases H} 
-| (a'::as) HD := 
-  begin
-    unfold list.filter, unfold ite, 
-    cases (HD a') with HD HD, simp, 
-    intro Ha, apply pred_of_mem_filter_pred, apply Ha,
-    intro Ha, cases Ha with Ha Ha, rewrite Ha, apply HD,
-    apply pred_of_mem_filter_pred, apply Ha
-  end 
 
 lemma ex_iff_ex (P Q : α → Prop) (H : ∀ a, P a ↔ Q a) : (∃ x, P x) ↔ (∃ x, Q x) :=
 begin
@@ -822,3 +125,28 @@ begin
   intro HP, cases HP with x Hx, 
   existsi x, apply (H x Hx)
 end
+
+def lcms : list nat → nat 
+| [] := 1
+| (n::ns) := nat.lcm n (lcms ns)
+
+def zlcms (zs : list int) : int :=
+lcms (list.map int.nat_abs zs)
+
+open tactic
+
+meta def papply pe := to_expr pe >>= apply  
+
+meta def intro_fresh : tactic expr :=
+get_unused_name `h none >>= tactic.intro 
+
+meta def intro_refl : tactic unit := 
+do t ← target, 
+   match t with 
+   | `(_ = _) := papply ``(eq.refl _)
+   | `(_ → _) := intro_fresh >> intro_refl
+   | _ := failed 
+   end
+
+meta def papply_trans (pe : pexpr) := 
+do papply ``(eq.trans), papply pe
