common/dnf.lean
@@ -16,8 +16,8 @@ def dnf : fm α → list (list α)
 | (fm.ex _) := []
 | (fm.not _) := []
 
-lemma dnf_prsv_normal [atom_type α β] : ∀ (p : fm α), 
-  fnormal β p → allp (allp (normal β)) (dnf p) 
+lemma dnf_prsv_pred [atom_type α β] (pr : α → Prop) : 
+  ∀ (φ : fm α), allp pr (@atoms _ (atom_type.dec_eq _ β) φ) → allp (allp pr) (dnf φ) 
 | (fm.true α) hnm := 
   begin
     intros as has, unfold dnf at has,
@@ -31,32 +31,43 @@ lemma dnf_prsv_normal [atom_type α β] : ∀ (p : fm α),
     rewrite exp_mem_singleton at has, 
     subst has, intros a' ha', 
     rewrite exp_mem_singleton at ha',
-    subst ha', apply hnm,
+    subst ha', apply hnm, apply or.inl rfl
   end
 | (fm.and p q) hnm := 
-  begin
-    unfold fnormal at hnm, cases hnm with hnmp hnmq,
+  begin 
+    unfold atoms at hnm,
+    rewrite exp_allp_union at hnm,
+    cases hnm with hnmp hnmq,
     unfold dnf, intros as has, intros a ha,
     rewrite exp_mem_map at has, 
     cases has with asp hasp, 
     cases hasp with hasp1 hasp2,
     cases asp with as1 as2, subst hasp2, 
     cases (mem_or_mem_of_mem_append ha) with hm hm,
-    apply dnf_prsv_normal p hnmp as1, 
+    apply dnf_prsv_pred p hnmp as1,  
     apply fst_mem_of_mem_product hasp1, apply hm,  
-    apply dnf_prsv_normal q hnmq as2, 
+    apply dnf_prsv_pred q hnmq as2, 
     apply snd_mem_of_mem_product hasp1, apply hm
   end
 | (fm.or p q) hnm := 
   begin
-    unfold fnormal at hnm, cases hnm with hnmp hnmq,
+    unfold atoms at hnm, 
+    rewrite exp_allp_union at hnm,
+    cases hnm with hnmp hnmq,
     unfold dnf, intros as has, intros a ha,
     cases (mem_or_mem_of_mem_append has) with hm hm,
-    apply dnf_prsv_normal p hnmp as hm a ha, 
-    apply dnf_prsv_normal q hnmq as hm a ha 
+    apply dnf_prsv_pred p hnmp as hm a ha, 
+    apply dnf_prsv_pred q hnmq as hm a ha 
   end
 | (fm.not _) hnm := allp_nil
 | (fm.ex _) hnm := allp_nil
+
+lemma dnf_prsv_normal [atom_type α β] : ∀ (p : fm α), 
+  fnormal β p → allp (allp (normal β)) (dnf p) := 
+begin
+  intros p hp, rewrite fnormal_iff_fnormal_alt at hp,
+  apply dnf_prsv_pred (normal β) _ hp, 
+end
 
 lemma dnf_prsv_alt [atom_type α β] : ∀ {p : fm α} {H : nqfree p} {xs : list β}, 
   disj_list (list.map (allp (atom_type.val xs)) (dnf p)) ↔ I p xs 
