presburger/cooper.lean
@@ -1,0 +1,38 @@
+import .correctness
+
+open pbgr
+
+def hd_coeff_one : int → atom → atom 
+| m (atom.le i (0::ks)) := (atom.le i (0::ks))   
+| m (atom.le i (k::ks)) := 
+  let m' := int.div m (abs k) in 
+  atom.le (m' * i) (int.sign k :: list.map (λ x, m' * x) ks)
+| m (atom.dvd d i (0::ks)) := (atom.dvd d i (0::ks)) 
+| m (atom.dvd d i (k::ks)) := 
+  let m' := int.div m k in 
+  atom.dvd (m' * d) (m' * i) (1 :: list.map (λ x, m' * x) ks)
+| m (atom.ndvd d i (0::ks)) := (atom.ndvd d i (0::ks)) 
+| m (atom.ndvd d i (k::ks)) := 
+  let m' := int.div m k in 
+  atom.ndvd (m' * d) (m' * i) (1 :: list.map (λ x, m' * x) ks)
+| m a := a
+
+def hd_coeffs_one (p : fm atom) : fm atom := 
+let m := zlcms (list.map hd_coeff (atoms_dep0 int p)) in 
+A' (atom.dvd m 0 [1]) ∧' (map_fm (hd_coeff_one m) p)
+
+def inf_minus : fm atom → fm atom 
+| ⊤' := ⊤' 
+| ⊥' := ⊥' 
+| (A' (atom.le i (k::ks))) := 
+  if k < 0 
+  then ⊤' 
+  else if k > 0
+       then ⊥' 
+       else A' (atom.le i (0::ks))
+| (A' a) := A' a
+| (p ∧' q) := and_o (inf_minus p) (inf_minus q)
+| (p ∨' q) := or_o (inf_minus p) (inf_minus q)
+| (¬' p) := ¬' p
+| (∃' p) := ∃' p
+
